CBS.Spec.fst
@@ -6,6 +6,7 @@ open FStar.Mul
 module U8 = FStar.UInt8
 
 
+// Speed up verification a bit.
 private
 val pow2_0_lemma: n:nat ->
   Lemma
@@ -14,6 +15,7 @@ val pow2_0_lemma: n:nat ->
     [SMTPat (pow2 n)]
 let pow2_0_lemma n = assert_norm(pow2 0 = 1)
 
+// Speed up verification a bit.
 private
 val pow2_8_lemma: n:nat ->
   Lemma
@@ -23,13 +25,31 @@ val pow2_8_lemma: n:nat ->
 let pow2_8_lemma n = assert_norm(pow2 8 = 256)
 
 
-let rec big_endian (b:seq U8.t) : Tot (n:nat) (decreases (Seq.length b)) =
+// Parse a given sequence of bytes in big-endian form, return a number.
+let rec big_endian (b:seq U8.t) : Tot (n:nat) (decreases (length b)) =
   if length b = 0 then 0
   else U8.v (last b) + pow2 8 * big_endian (slice b 0 (length b - 1))
 
 
+// Speed up verification a bit.
 private
-val big_endian_zero: (b:seq U8.t) -> Lemma
+val lemma_big_endian_0: (b:seq U8.t) -> Lemma
   (ensures (big_endian (slice b 0 0) = 0))
   [SMTPat (big_endian (slice b 0 0))]
-let big_endian_zero b = ()
+let lemma_big_endian_0 b = ()
+
+
+// Ensure that big_endian always returns a number
+// smaller than 2^(n*8) for a sequence of length n.
+private
+val lemma_big_endian_bounds: (b:seq U8.t) -> Lemma
+  (ensures (big_endian b < pow2 (length b * 8)))
+  (decreases (length b))
+  [SMTPat (big_endian b < pow2 (length b * 8))]
+let rec lemma_big_endian_bounds b =
+  let len = length b in
+    if len > 0 then (
+      lemma_big_endian_bounds (slice b 0 (len - 1));
+      Math.Lemmas.pow2_minus (len * 8) ((len - 1) * 8);
+      ()
+    )
