CBS.fst
@@ -17,7 +17,7 @@ module ST = FStar.HyperStack.ST
 #reset-options "--max_fuel 5 --z3rlimit 100"
 
 
-private
+private // TODO describe
 noeq type cbs_t = | MkCBS: data:(buffer U8.t) -> len:U32.t{U32.v len == length data} -> cbs_t
 
 private inline_for_extraction
@@ -27,22 +27,32 @@ private inline_for_extraction
 let u32_to_u16 n = FStar.Int.Cast.uint32_to_uint16 n
 
 
+// Generic function used to specify pre-conditions for `cbs_get_u*` functions.
+[@ "substitute"] private
+let cbs_precond cbs out = fun h ->
+  // `cbs` and `out` should be normal pointers.
+  length cbs = 1 /\ length out = 1 /\
+  (let data = (get h cbs 0).data in (
+    // Ensure that `cbs_t *cbs`, `cbs->data`, and `uintX_t *out` are live.
+    live h cbs /\ live h data /\ live h out /\
+    // Ensure that none of the above memory areas intersect.
+    disjoint cbs out /\ disjoint out data /\ disjoint cbs data
+  ))
+
+
 // bool cbs_get_u(cbs_t *cbs, uint32_t *out, uint32_t num)
-// TODO check that 0 <= num < 5
 val cbs_get_u :
-  cbs: buffer cbs_t{length cbs = 1} -> // TODO cbs_p ?
-  out: buffer U32.t{length out = 1 /\ disjoint out cbs} -> // TODO uint32_p ?
+  cbs: buffer cbs_t{length cbs = 1} ->
+  out: buffer U32.t{length out = 1} ->
+  // TODO check that 0 <= num < 5
   num: U32.t{U32.(v num > 0 /\ v num < 5)} ->
   ST bool
-  (requires (fun h -> live h out /\ live h cbs /\ live h (get h cbs 0).data
-    /\ disjoint out (get h cbs 0).data /\ disjoint cbs (get h cbs 0).data // TODO
-  ))
+  (requires (cbs_precond cbs out))
   (ensures (fun h0 r h1 -> live h0 out /\ live h1 out /\ modifies_1 out h0 h1 /\
     (let cbs0 = get h0 cbs 0 in
       // Return false if there aren't enough bytes.
       r == U32.(v cbs0.len >= v num) /\
       // If there are, check the result.
-      // TODO make this a function
       (r ==> U32.v (get h1 out 0) == big_endian (slice (as_seq h0 cbs0.data) 0 (U32.v num))) /\
       // The result must be < 2^(num * 8).
       (r ==> U32.v (get h1 out 0) < pow2 (U32.v num * 8)) // TODO formatting
@@ -53,7 +63,7 @@ let cbs_get_u cbs out num =
   let h0 = ST.get() in
   if U32.(cbs0.len >=^ num) then (
     let inv = (fun h i -> live h out /\ live h cbs0.data /\ modifies_1 out h0 h
-      /\ 0 <= i /\ i <= U32.v num // TODO comments
+      /\ 0 <= i /\ i <= U32.v num // TODO comments, functions?
       /\ U32.v (get h out 0) < pow2 (i * 8)
       /\ U32.v (get h out 0) == big_endian (slice (as_seq h0 cbs0.data) 0 i)
     ) in
@@ -81,11 +91,9 @@ let cbs_get_u cbs out num =
 // bool cbs_get_u8(cbs_t *cbs, uint8_t *out)
 val cbs_get_u8 :
   cbs: buffer cbs_t{length cbs = 1} ->
-  out: buffer U8.t{length out = 1 /\ disjoint out cbs} ->
+  out: buffer U8.t{length out = 1} ->
   ST bool
-  (requires (fun h -> live h cbs /\ live h out /\ live h (get h cbs 0).data
-    /\ disjoint out (get h cbs 0).data /\ disjoint cbs (get h cbs 0).data
-  ))
+  (requires (cbs_precond cbs out))
   (ensures (fun h0 r h1 -> live h1 out /\ modifies_1 out h0 h1 /\
     (let cbs0 = get h0 cbs 0 in
       // Return false if there aren't enough bytes.
@@ -107,11 +115,9 @@ let cbs_get_u8 cbs out =
 // bool cbs_get_u16(cbs_t *cbs, uint16_t *out)
 val cbs_get_u16 :
   cbs: buffer cbs_t{length cbs = 1} ->
-  out: buffer U16.t{length out = 1 /\ disjoint out cbs} ->
+  out: buffer U16.t{length out = 1} ->
   ST bool
-  (requires (fun h -> live h out /\ live h cbs /\ live h (get h cbs 0).data
-    /\ disjoint out (get h cbs 0).data /\ disjoint cbs (get h cbs 0).data
-  ))
+  (requires (cbs_precond cbs out))
   (ensures (fun h0 r h1 -> live h1 out /\ modifies_1 out h0 h1 /\
     (let cbs0 = get h0 cbs 0 in
       // Return false if there aren't enough bytes.
@@ -133,19 +139,17 @@ let cbs_get_u16 cbs out =
 // bool cbs_get_u24(cbs_t *cbs, uint32_t *out)
 val cbs_get_u24 :
   cbs: buffer cbs_t{length cbs = 1} ->
-  out: buffer U32.t{length out = 1 /\ disjoint out cbs} ->
+  out: buffer U32.t{length out = 1} ->
   ST bool
-  (requires (fun h -> live h out /\ live h cbs /\ live h (get h cbs 0).data
-    /\ disjoint out (get h cbs 0).data /\ disjoint cbs (get h cbs 0).data
-  ))
+  (requires (cbs_precond cbs out))
   (ensures (fun h0 r h1 -> live h1 out /\ modifies_1 out h0 h1 /\
     (let cbs0 = get h0 cbs 0 in
       // Return false if there aren't enough bytes.
       r == (U32.v cbs0.len > 2) /\
       // If there are, check the result.
-      (r ==> U32.v (get h1 out 0) == big_endian (slice (as_seq h0 cbs0.data) 0 3))
+      (r ==> U32.v (get h1 out 0) == big_endian (slice (as_seq h0 cbs0.data) 0 3)) /\
       // The result must be < 2^24.
-      /\ (r ==> U32.v (get h1 out 0) < pow2 24) // TODO formatting
+      (r ==> U32.v (get h1 out 0) < pow2 24) // TODO formatting
     )))
 
 let cbs_get_u24 cbs out =
@@ -155,11 +159,9 @@ let cbs_get_u24 cbs out =
 // bool cbs_get_u32(cbs_t *cbs, uint32_t *out)
 val cbs_get_u32 :
   cbs: buffer cbs_t{length cbs = 1} ->
-  out: buffer U32.t{length out = 1 /\ disjoint out cbs} ->
+  out: buffer U32.t{length out = 1} ->
   ST bool
-  (requires (fun h -> live h out /\ live h cbs /\ live h (get h cbs 0).data
-    /\ disjoint out (get h cbs 0).data /\ disjoint cbs (get h cbs 0).data
-  ))
+  (requires (cbs_precond cbs out))
   (ensures (fun h0 r h1 -> live h1 out /\ modifies_1 out h0 h1 /\
     (let cbs0 = get h0 cbs 0 in
       // Return false if there aren't enough bytes.
